\section{2nd Derivative BackProp Weight Update Rule}
Weight error (1st order approx):
\begin{align}
E\left(w\right) &= E\left(w_0\right) + \pdv{E}{w}\left(w - w_0\right)
\end{align}
We want:
\begin{align}
E\left(w\right) &= 0
\end{align}
\begin{align}
0 &= E\left(w_0\right) + \pdv{E}{w}\left(w - w_0\right)
\\
0 &= E\left(w_0\right) + \pdv{E}{w}w - \pdv{E}{w}w_0
\\
\pdv{E}{w}w  &= \pdv{E}{w}w_0 - E\left(w_0\right)
\\
w  &= w_0 - \frac{E\left(w_0\right)}{\pdv{E}{w}} 
\end{align}
Weight error (2nd order approx):
\begin{align}
E\left(w\right) &= E\left(w_0\right) + \pdv{E}{w}\left(w - w_0\right) + \frac{1}{2}\pdv[2]{E}{w}\left(w - w_0\right)^2
\end{align}
We want:
\begin{align}
E\left(w\right) &= 0
\end{align}
\begin{align}
0 &= 
\underbrace{E\left(w_0\right)}
_{c}
+ 
\underbrace{\pdv{E}{w}}
_{b} 
\left(w - w_0\right)
+ 
\underbrace{\frac{1}{2}\pdv[2]{E}{w}}
_{a}
\left(w - w_0\right)^2
\\
0 &= ax^2 + bx + c \\
x &= \frac{-b \pm \sqrt{b^2 - 4ac}}{2a}
\\
\left(w - w_0\right) &= \frac{-\left(\pdv{E}{w}\right) \pm \sqrt{\left(\pdv{E}{w}\right)^2 - 4\left(\frac{1}{2}\pdv[2]{E}{w}\right)E\left(w_0\right)}}{2\left(\frac{1}{2}\pdv[2]{E}{w}\right)}
\\
w &= w_0 + \frac{-\left(\pdv{E}{w}\right) \pm \sqrt{\left(\pdv{E}{w}\right)^2 - 2\left(\pdv[2]{E}{w}\right)E\left(w_0\right)}}{\left(\pdv[2]{E}{w}\right)}
\end{align}
We only need one of the zeros so...
\begin{align}
w &= w_0 + \frac{\sqrt{\left(\pdv{E}{w}\right)^2 - 2\left(\pdv[2]{E}{w}\right)E\left(w_0\right)} + \left(\pdv{E}{w}\right)}{\left(\pdv[2]{E}{w}\right)}
\end{align}